example_userbase.thy
@@ -59,7 +59,7 @@ datatype userDataOp =
 
 instance userDataOp :: countable
   by countable_datatype
-instantiation userDataOp ::  valueType begin
+instantiation userDataOp :: crdt_op begin
 definition "uniqueIds_userDataOp x \<equiv> 
   case x of 
      Name x \<Rightarrow> uniqueIds x
@@ -70,6 +70,8 @@ lemma [simp]: "uniqueIds (Name x) = uniqueIds x"
   by (auto simp add: uniqueIds_userDataOp_def)
 
 definition [simp]: "default_userDataOp = Mail default"
+
+definition "is_update_userDataOp x \<equiv> case x of Name x \<Rightarrow> is_update x | Mail x \<Rightarrow> is_update x"
 
 instance by (standard, auto)
 end
@@ -185,8 +187,9 @@ definition inv2  where
 
 definition inv3  where
   "inv3 c_calls hb \<equiv> \<not>(\<exists>write delete u upd.
-    (c_calls write \<triangleq> Call (NestedOp u upd) Undef)
-  \<and> (c_calls delete \<triangleq> Call (DeleteKey u) Undef)
+    (\<exists>write_r. c_calls write \<triangleq> Call (NestedOp u upd) write_r)
+  \<and> is_update upd
+  \<and> (\<exists>delete_r. c_calls delete \<triangleq> Call (DeleteKey u) delete_r)
   \<and> (delete, write) \<in> hb
   )"
 
@@ -202,6 +205,16 @@ lemma show_inv[intro, case_names inv1 inv2 inv3]:
     and "inv3 (calls ctxt) (happensBefore ctxt)"
   shows "inv ctxt"
   using assms  by (auto simp add: inv_def)
+
+lemma use_inv3:
+  assumes "inv3 c_calls hb"
+and "c_calls write \<triangleq> Call (NestedOp u upd) write_r"
+and "is_update upd"
+and "c_calls delete \<triangleq> Call (DeleteKey u) delete_r"
+and "(delete, write) \<in> hb"
+shows P
+  by (meson assms inv3_def)
+
 
 definition userStruct :: "(userDataOp, val) crdtSpec" where
   "userStruct \<equiv> (\<lambda>oper.
@@ -223,6 +236,8 @@ definition progr :: "(proc, localState, operation, val) prog" where
 lemma procedure_progr[simp]: "procedure progr = procedures"
   by (simp add: progr_def)
 
+lemma querySpec_progr[simp]: "querySpec progr = crdtSpec"
+  by (simp add: progr_def)
 
 
 
@@ -257,8 +272,8 @@ proof (auto simp add: program_wellFormed_def)
       by (auto simp add: getUser_impl_def, show_procedures_cannot_guess_ids  )
   qed
 
-  show "queries_cannot_guess_ids (querySpec progr)"
-  proof (simp add: progr_def crdtSpec_def, standard)
+  show "queries_cannot_guess_ids crdtSpec"
+  proof (simp add:  crdtSpec_def, standard)
     show "queries_cannot_guess_ids userStruct"
     proof (auto simp add: userStruct_def queries_cannot_guess_ids_def split: userDataOp.splits)
 
@@ -358,7 +373,7 @@ proof M_show_programCorrect
         case execution
         show "execution_s_correct progr S i"
           using procedure_correct.in_initial_state
-        proof (fuzzy_rule execution_s_check_sound2)
+        proof (fuzzy_rule execution_s_check_sound3)
 
 
 
@@ -370,22 +385,20 @@ proof M_show_programCorrect
 
           note registerUser_impl_def[simp]
 
+          show "invocationOp S i \<triangleq> RegisterUser name mail"
+            using RegisterUser \<open>invocationOp S i \<triangleq> proc\<close> by blast
 
 
 
-          show "execution_s_check progr i s_calls s_happensBefore s_callOrigin s_transactionOrigin
-            s_knownIds s_invocationOp s_invocationRes {} {} {} [] None True
-            (registerUser_impl (String name) (String mail))"
-            if "s_invocationOp i = invocationOp S i"
-              and "s_invocationRes i = None"
+          show "execution_s_check progr i s_calls s_happensBefore s_callOrigin s_transactionOrigin s_knownIds
+              (s_invocationOp(i \<mapsto> RegisterUser name mail)) (s_invocationRes(i := None)) {} {} {} [] None True
+              (registerUser_impl (String name) (String mail))"
             for s_calls s_happensBefore s_callOrigin s_transactionOrigin s_knownIds s_invocationOp s_invocationRes
           proof (repliss_vcg, goal_cases "AtCommit" "AtReturn" )
             case (AtCommit v tx s_calls' s_happensBefore' s_callOrigin' s_transactionOrigin' s_knownIds' vis' s_invocationOp' s_invocationRes' c res ca resa)
 
             find_theorems uid_is_private
 
-            have my_invoc[simp]: "s_invocationOp' i \<triangleq> RegisterUser name mail"
-              by (simp add: AtCommit that(1) RegisterUser)
 
 
             have v_no_op: "to_nat v \<notin> uniqueIds op" if "s_calls c \<triangleq> Call op r" for c op r
@@ -436,6 +449,7 @@ proof M_show_programCorrect
               show ?case
                 by (auto simp add: inv1_def)
 
+
             next
               case inv2
               from `inv2 s_invocationOp' (i_callOriginI_h s_callOrigin' s_transactionOrigin') s_calls'`
@@ -446,9 +460,23 @@ proof M_show_programCorrect
                 done 
             next 
               case inv3
+
+              from `uid_is_private' i s_calls' s_invocationOp' s_invocationRes' s_knownIds' (to_nat v)`
+              have "new_unique_not_in_calls s_calls' (to_nat v)"
+                by (auto simp add: uid_is_private'_def)
+
+
+              text "Because v is a new unique id there can be no delete operation on that type:"
+              hence no_delete: "s_calls' delete \<noteq> Some (Call (DeleteKey v) delete_r)" for delete delete_r
+                using `uniqueIds v = {to_nat v}` by (auto simp add: new_unique_not_in_calls_def uniqueIds_mapOp_def, force)
+
+                
+
               from `inv3 s_calls' s_happensBefore'`
               show ?case
-                by (auto simp add: inv3_def `c \<noteq> ca` updateHb_cases in_sequence_cons inv3(19) v_no_delete2')
+                by (auto simp add: no_delete inv3_def `c \<noteq> ca` updateHb_cases in_sequence_cons inv3(17) inv3(19) v_no_delete2')
+                
+
 
             qed
 
@@ -460,24 +488,155 @@ proof M_show_programCorrect
             then show ?case
               apply (auto simp add: inv_def)
               apply (auto simp add: inv1_def)
-              apply (metis RegisterUser \<open>invocationOp S i \<triangleq> proc\<close> option.inject proc.distinct(5) that(1))
-              apply (metis RegisterUser \<open>invocationOp S i \<triangleq> proc\<close> option.inject proc.distinct(5) that(1))
               done
           qed
 
-          show "initialStates' progr i = initialStates progr i"
-            by (simp add: initialStates'_same)
         qed
       qed
 
     next
-      case (UpdateMail x21 x22)
+      case (UpdateMail user mail)
+
+      show "procedureCorrect progr S i"
+      proof M_show_procedureCorrect
+        case after_invocation
+        show ?case 
+          using show_P.invariant_pre UpdateMail
+          by (auto simp add:  inv_def inv1_def inv2_def inv3_def invContextH2_simps)
+
+      next
+        case execution
+        show "execution_s_correct progr S i"
+          using procedure_correct.in_initial_state
+        proof (fuzzy_rule execution_s_check_sound3)
+
+
+
+          show "currentProc S i \<triangleq> toImpl"
+            by (auto simp add: UpdateMail procedures_def )
+
+          show "localState S i \<triangleq> updateMail_impl (UserId user) (String mail)"
+            by (auto simp add: UpdateMail procedures_def )
+
+          note updateMail_impl_def[simp]
+
+          show "invocationOp S i \<triangleq> UpdateMail user mail"
+            using UpdateMail \<open>invocationOp S i \<triangleq> proc\<close> by blast
+
+
+
+          show "execution_s_check progr i s_calls s_happensBefore s_callOrigin s_transactionOrigin s_knownIds
+              (s_invocationOp(i \<mapsto> UpdateMail user mail)) (s_invocationRes(i := None)) {} {} {} [] None True
+              (updateMail_impl (UserId user) (String mail))"
+            for  s_calls s_happensBefore s_callOrigin s_transactionOrigin s_knownIds s_invocationOp s_invocationRes
+          proof ((repliss_vcg; intro conjI impI; repliss_vcg?), goal_cases "Exists_AtCommit" "Exists_AtReturn" "NotExists_AtCommit" "NotExists_AtReturn"  )
+            case (Exists_AtCommit tx s_calls' s_happensBefore' s_callOrigin' s_transactionOrigin' s_knownIds' vis' s_invocationOp' s_invocationRes' c res ca resa)
+            
+            from Exists_AtCommit
+            show ?case
+            proof (auto simp add: inv_def, goal_cases inv1 inv2 inv3)
+              case inv1
+              
+              from `inv1 s_invocationOp' s_invocationRes'(invocation_happensBeforeH (i_callOriginI_h s_callOrigin' s_transactionOrigin') s_happensBefore')`
+              show ?case
+                by (auto simp add: inv1_def) 
+
+            next
+              case inv2
+              from `inv2 s_invocationOp' (i_callOriginI_h s_callOrigin' s_transactionOrigin') s_calls'`
+              show ?case
+               using `c \<noteq> ca` by (auto simp add: inv2_def i_callOriginI_h_update_to3)
+            next
+              case inv3
+
+              from \<open>crdtSpec (KeyExists (UserId user)) \<lparr>calls = s_calls' |` vis', happensBefore = s_happensBefore' |r vis'\<rparr> (Bool True)\<close>
+                obtain upd_c upd_op upd_r 
+                  where c0: "upd_c \<in> vis'"
+                    and c1: "is_update upd_op"
+                    and c2: "s_calls' upd_c \<triangleq> Call (NestedOp (UserId user) upd_op) upd_r"
+                    and c3: "\<forall>c'. c' \<in> vis' \<longrightarrow> (\<forall>r. s_calls' c' \<noteq> Some (Call (DeleteKey (UserId user)) r)) \<or> (c', upd_c) \<in> s_happensBefore'"
+                  by (auto simp add: crdtSpec_def map_dw_spec_def map_spec_def deleted_calls_dw_def restrict_relation_def restrict_map_def split: if_splits)
+
+
+                show ?case
+                proof (auto simp add: inv3_def `c \<noteq> ca` `c \<noteq> ca`[symmetric])
+
+                  show "False"
+                    if d3: "is_update (Mail (Assign (String mail)))"
+                      and d0: "delete \<noteq> c"
+                      and d1: "delete \<noteq> ca"
+                      and d5: "(delete, ca) \<in> updateHb s_happensBefore' vis' [c, ca]"
+                      and d2: "s_calls' delete \<triangleq> Call (DeleteKey (UserId user)) delete_r"
+                    for  delete delete_r
+                  proof -
+                    from d5
+                    have "delete \<in> vis'"
+                      by (auto simp add: updateHb_cases in_sequence_cons inv3(13) d0[symmetric])
+
+                    from c3[rule_format, OF `delete \<in> vis'`]
+                    have "(delete, upd_c) \<in> s_happensBefore'"
+                      by (auto simp add: d2)
+
+                    text "This violates invariant 3"
+                    with `inv3 s_calls' s_happensBefore'` c2 c1 d2
+                    show False
+                      apply (auto simp add: inv3_def)
+                      by blast
+                  qed
+
+                  show "False"
+                    if d0: "write \<noteq> c"
+                      and d1: "write \<noteq> ca"
+                      and d2: "delete \<noteq> c"
+                      and d3: "delete \<noteq> ca"
+                      and d4: "is_update upd"
+                      and d5: "s_calls' write \<triangleq> Call (NestedOp u upd) write_r"
+                      and d6: "(delete, write) \<in> updateHb s_happensBefore' vis' [c, ca]"
+                      and d7: "s_calls' delete \<triangleq> Call (DeleteKey u) delete_r"
+                    for "write" delete u upd write_r delete_r
+                  proof - text "From old invariant ... "
+                    from d6
+                    have "(delete, write) \<in> s_happensBefore'"
+                      by (metis d0 d1  insert_iff list.set(1) list.simps(15) singletonD updateHb_simp2)
+
+
+                    with `inv3 s_calls' s_happensBefore'` d4 d5 d7 
+                    show False
+                      by (auto simp add: inv3_def, blast)
+
+                  qed
+                qed
+              qed
+
+            next
+              case (Exists_AtReturn tx s_calls' s_happensBefore' s_callOrigin' s_transactionOrigin' s_knownIds' vis' s_invocationOp' s_invocationRes' c res ca resa)
+              then show ?case
+                by (auto simp add: inv_def inv1_def) 
+            next
+              case (NotExists_AtCommit tx s_calls' s_happensBefore' s_callOrigin' s_transactionOrigin' s_knownIds' vis' s_invocationOp' s_invocationRes' c res)
+
+              
+
+
+              
+              from NotExists_AtCommit
+              show ?case 
+                by (auto simp add: inv_def inv1_def inv2_def inv3_def 
+                      i_callOriginI_h_update_to3 map_update_all_get updateHb_single)
+
+            next
+              case (NotExists_AtReturn tx s_calls' s_happensBefore' s_callOrigin' s_transactionOrigin' s_knownIds' vis' s_invocationOp' s_invocationRes' c res)
+              then show ?case 
+                by (auto simp add: inv_def inv1_def) 
+            qed
+          qed
+        qed
+
+    next
+      case (RemoveUser user)
       then show ?thesis sorry
     next
-      case (RemoveUser x3)
-      then show ?thesis sorry
-    next
-      case (GetUser x4)
+      case (GetUser user)
       then show ?thesis sorry
     qed
   qed
